Finish equivalence proof, fix regexp translation along the way

warblreequiv/RegexpTranslation.v
@@ -27,7 +27,7 @@ Inductive equiv_quantifier: Patterns.QuantifierPrefix -> (bool -> regex -> regex
 | Equiv_star: equiv_quantifier Patterns.Star (fun greedy => Quantified greedy 0 +∞)
 | Equiv_plus: equiv_quantifier Patterns.Plus (fun greedy => Quantified greedy 1 +∞)
 | Equiv_question: equiv_quantifier Patterns.Question (fun greedy => Quantified greedy 0 (NoI.N 1))
-| Equiv_repexact: forall n, equiv_quantifier (Patterns.RepExact n) (fun greedy => Quantified greedy n (NoI.N n))
+| Equiv_repexact: forall n, equiv_quantifier (Patterns.RepExact n) (fun greedy => Quantified greedy n (NoI.N 0))
 | Equiv_reppartialrange: forall n, equiv_quantifier (Patterns.RepPartialRange n) (fun greedy => Quantified greedy n +∞)
 | Equiv_reprange: forall mini maxi, mini <= maxi -> equiv_quantifier (Patterns.RepRange mini maxi) (fun greedy => Quantified greedy mini (NoI.N (maxi-mini))).
 
